theories/factorial/factorial_modified.v
@@ -1,0 +1,153 @@
+(*Preamble*)
+Require Import Volpic_preamble.
+Require Import Volpic_notation.
+Require Import String.
+Require Import ZArith.
+Require Import List.
+Require Import Bool.
+Open Scope string_scope.
+Open Scope Z_scope.
+Open Scope volpic_notation.
+Import ListNotations.
+
+Definition factorial (VP_store: store) loop_limit := 
+	let VP_poison := false in
+	let (VP_store,VP_poison) := 
+		(if (negb VP_poison) then
+ 			 (update VP_store "VP_result" (VInteger ( 1 )),VP_poison) 
+		else
+ 			(VP_store,true)) in
+	let (VP_store,VP_poison) := 
+		(if (negb VP_poison) then
+			match 
+				while ( fun VP_store => 1 <=? get_int VP_store "VP_X" ) with VP_store upto loop_limit begin fun VP_store => (*Block: next 2 statements*)
+					let VP_store := update VP_store "VP_result" (VInteger ( get_int VP_store "VP_result" * get_int VP_store "VP_X" )) in
+					update VP_store "VP_X" (VInteger ( get_int VP_store "VP_X" - 1 )) 
+				end
+			with 
+			| None => (VP_store, true)
+			| Some s => (s, VP_poison)
+			end
+		else
+ 			(VP_store,true)) in
+	(VP_store, VP_poison).
+
+Definition output_safe (f : store -> nat -> store * bool) 
+		input expected :=
+	forall loop_limit output, 
+		(output, false) = f input loop_limit -> output "VP_result" = expected.
+
+Ltac vpex_term term := 
+	match term with [(?fst, ?snd) = 
+			match ?m with (Some s) => ?s' | None => ?n' end] => idtac s
+	end.
+
+Ltac vpex :=
+	match goal with [H: (?fst, ?snd) = 
+		match ?m with (Some s) => ?s' | None => ?n' end |- _] =>
+			let name := fresh "body" in
+			remember m as name
+		| [H: (?fst, ?snd) = (let (st, ps) := 
+			match ?m with (Some s) => ?s' | None => ?n' end in _) |- _] =>
+			let E := fresh "E" in 
+			destruct m eqn:E
+	end || idtac "No match".
+
+Require Import FunctionalExtensionality.
+
+Lemma update_shadow : forall (m : store) x v1 v2,
+  (x !-> v2 ; x !-> v1 ; m) = (x !-> v2 ; m).
+Proof.
+  intros. apply functional_extensionality. intros.
+  unfold update. destruct (String.eqb x0 x) eqn:E; reflexivity.
+Qed.
+
+Lemma update_eq : forall (m : store) x v,
+	(x !-> v; m) x = v.
+Proof.
+	intros. unfold update. now rewrite String.eqb_refl.
+Qed.
+
+Lemma update_neq : forall (m : store) x y v,
+	x <> y ->
+	(x !-> v; m) y = m y.
+Proof.
+	intros. unfold update. destruct (eqb_neq x y). now rewrite String.eqb_sym, (H1 H).
+Qed.
+
+Theorem update_permute : 
+  forall (m : store)
+    v1 v2 x1 x2,
+  x2 <> x1 ->
+  (x1 !-> v1 ; x2 !-> v2 ; m)
+  =
+  (x2 !-> v2 ; x1 !-> v1 ; m).
+Proof.
+  intros. apply functional_extensionality. intros.
+  unfold update. destruct (x =? x1)%string eqn:E, (x =? x2)%string eqn:E'; auto.
+  pose (String.eqb_eq x x1). pose (String.eqb_eq x x2).
+  destruct i, i0. specialize (H0 E). specialize (H2 E'). subst. contradiction.
+Qed.
+
+Definition Z_fact (n : Z) := Z.of_nat (fact (Z.to_nat n)).
+
+Lemma fact_sub : forall n,
+	(1 <= n)%nat ->
+	fact n = (n * fact (n - 1))%nat.
+Proof.
+	induction n; intros; simpl in *.
+	inversion H. now rewrite Nat.sub_0_r.
+Qed.
+
+Require Import Lia.
+
+Lemma Z_fact_sub : forall n,
+	1 <= n ->
+	Z_fact n = n * Z_fact (n - 1).
+Proof.
+	intros. replace n with (Z.of_nat (Z.to_nat n)).
+	unfold Z_fact. rewrite Nat2Z.id. 
+		replace (Z.of_nat (Z.to_nat n) - 1) with (Z.of_nat (Z.to_nat (n - 1))). 
+		rewrite Nat2Z.id. 
+		rewrite <- Nat2Z.inj_mul, Z2Nat.inj_sub. replace (Z.to_nat 1) with 1%nat. 
+		rewrite fact_sub; lia. all: lia.
+Qed.
+
+Lemma nle_1_destruct : forall n,
+	~ (1 <= n) ->
+	n = 0 \/ exists p, n = Z.neg p.
+Proof.
+	intros.	destruct n; try lia.
+	right. now exists p.
+Qed.
+
+Lemma Z_fact_nle_1 : forall n,
+	(1 <=? n) = false ->
+	Z_fact n = 1.
+Proof.
+	intros. apply Z.leb_nle in H. apply nle_1_destruct in H. destruct H; subst.
+	reflexivity. destruct H. subst. reflexivity.
+Qed.
+
+Theorem factorial_correct : forall n,
+	output_safe factorial ("VP_X" !-> VInteger n; fresh_store) (VInteger (Z_fact n)).
+Proof.
+	intros n loop_limit output Terminates. unfold factorial in Terminates. simpl in Terminates.
+		vpex. inversion Terminates; subst; clear Terminates. 
+		generalize dependent s. replace (Z_fact n) with (1 * Z_fact n).
+		generalize dependent n. generalize 1 at 3 4 as inter_prod.
+		induction loop_limit; intros.
+			inversion E. match goal with [H: forall i n s, ?x ?l ?b ?store = _ -> _ |- _] => 
+				remember x as loop_body end.
+			simpl in *. unfold get_int in E.
+				rewrite update_neq, update_eq, update_eq, update_neq, update_neq, update_eq in E;
+					try discriminate. destruct (1 <=? n) eqn:E0.
+			rewrite update_shadow, update_permute, update_shadow in E; try discriminate.
+			rewrite (IHloop_limit _ _ _ E).
+			rewrite Heqloop_body in E. destruct loop_limit. inversion E. simpl in E.
+			unfold get_int in E. rewrite update_eq in E.
+			rewrite <- Z.mul_assoc, <- Z_fact_sub. reflexivity. lia.
+			inversion E; subst. rewrite update_eq.
+			rewrite (Z_fact_nle_1 _ E0). now rewrite Z.mul_1_r. lia.
+		inversion Terminates.
+Qed.
