theories/factorial/factorial.p
@@ -1,0 +1,25 @@
+program Factorial;
+
+uses
+    sysutils;
+
+function factorial(x: integer) : integer;
+begin
+    factorial := 1;
+    while 1 <= x do
+    begin
+        factorial := factorial * x;
+        x := x - 1;
+    end;
+end;
+
+var 
+    i : string;
+    n : integer;
+begin
+    write('n: ');
+    readln(i);
+    n := strtoint(i);
+
+    writeln('fact(n): ', factorial(n));
+end.
